# Homework 1

Iowa State University Astrodynamics I (AERE 351) Homework 1

## Problem 1.1

Given:

$$
\begin{align*}
  A &= A_x \hat{i} + A_y \hat{j} + A_z \hat{k} \\

  B &= B_x \hat{i} + B_y \hat{j} + B_z \hat{k} \\

  C &= C_x \hat{i} + C_y \hat{j} + C_z \hat{k}
\end{align*}
$$

### a.

Given:

$$
A \cdot A = |A|^2
$$

Left hand side:

$$
\begin{align*}
  A \cdot A &= A_x \cdot A_x + A_y \cdot A_y + A_z \cdot A_z \\

  &= \boxed{A_x^2 + A_y^2 + A_z^2}
\end{align*}
$$

Right hand side:

$$
\begin{align*}
  |A|^2 &= \left[ \sqrt{A_x^2 + A_y^2 + A_z^2} \right]^2 \\

  &= \boxed{A_x^2 + A_y^2 + A_z^2}
\end{align*}
$$

### b.

Given:

$$
A \cdot (B \times C) = (A \times B) \cdot C
$$

Left hand side:

$$
\begin{align*}
  A \cdot (B \times C) &= A \cdot
    \begin{vmatrix}
      \hat{i} & \hat{j} & \hat{k} \\
      B_x & B_y & B_z \\
      C_x & C_y & C_z
    \end{vmatrix} \\

  &= A \cdot \left[ (B_y C_z - B_z C_y) \hat{i} + (B_z C_x - B_x C_z) \hat{j} + (B_x C_y - B_y C_x) \hat{k} \right] \\

  &= \boxed{A_x B_y C_z - A_x B_z C_y + A_y B_z C_x - A_y B_x C_z + A_z B_x C_y - A_z B_y C_x}
\end{align*}
$$

Right hand side:

$$
\begin{align*}
  (A \times B) \cdot C &=
    \begin{vmatrix}
      \hat{i} & \hat{j} & \hat{k} \\
      A_x & A_y & A_z \\
      B_x & B_y & B_z
    \end{vmatrix} \cdot C \\

  &= \left[ (A_y B_z - A_z B_y) \hat{i} + (A_z B_x - A_x B_z) \hat{j} + (A_x B_y - A_y B_x) \hat{k} \right] \cdot C \\

  &= A_y B_z C_x - A_z B_y C_x + A_z B_x C_y - A_x B_z C_y + A_x B_y C_z - A_y B_x C_z \\

  &= \boxed{A_x B_y C_z - A_x B_z C_y + A_y B_z C_x - A_y B_x C_z + A_z B_x C_y - A_z B_y C_x}
\end{align*}
$$

### c.

Given:

$$
A \times (B \times C) = B (A \cdot C) - C (A \cdot B)
$$

Left hand side:

$$
\begin{align*}
  A \times (B \times C) &= A \times
    \begin{vmatrix}
      \hat{i} & \hat{j} & \hat{k} \\
      B_x & B_y & B_z \\
      C_x & C_y & C_z
    \end{vmatrix} \\

  &= A \times \left[ (B_y C_z - B_z C_y) \hat{i} + (B_z C_x - B_x C_z) \hat{j} + (B_x C_y - B_y C_x) \hat{k} \right] \\

  &=
    \begin{vmatrix}
      \hat{i} & \hat{j} & \hat{k} \\
      A_x               & A_y               & A_z \\
      B_y C_z - B_z C_y & B_z C_x - B_x C_z & B_x C_y - B_y C_x
    \end{vmatrix} \\

  &= \boxed{
    \begin{bmatrix}
      A_y B_x C_y - A_y B_y C_x - A_z B_z C_x + A_z B_x C_z \\
      A_z B_y C_z - A_z B_z C_y - A_x B_x C_y + A_x B_y C_x \\
      A_x B_z C_x - A_x B_x C_z - A_y B_y C_z + A_y B_z C_y
    \end{bmatrix}
  }
\end{align*}
$$

Right hand side:

$$
\begin{align*}
  B (A \cdot C) - C (A \cdot B) &= B (A_x C_x + A_y C_y + A_z C_z) - C (A_x B_x + A_y B_y + A_z B_z) \\

  &= \begin{bmatrix}
    B_x A_x C_x + B_x A_y C_y + B_x A_z C_z \\
    B_y A_x C_x + B_y A_y C_y + B_y A_z C_z \\
    B_z A_x C_x + B_z A_y C_y + B_z A_z C_z
  \end{bmatrix} - \\
  &\quad~ \begin{bmatrix}
    C_x A_x B_x + C_x A_y B_y + C_x A_z B_z \\
    C_y A_x B_x + C_y A_y B_y + C_y A_z B_z \\
    C_z A_x B_x + C_z A_y B_y + C_z A_z B_z
  \end{bmatrix} \\

  &= \begin{bmatrix}
    A_x B_x C_x + A_y B_x C_y + A_z B_x C_z \\
    A_x B_y C_x + A_y B_y C_y + A_z B_y C_z \\
    A_x B_z C_x + A_y B_z C_y + A_z B_z C_z
  \end{bmatrix} - \\
  &\quad~ \begin{bmatrix}
    A_x B_x C_x + A_y B_y C_x + A_z B_z C_x \\
    A_x B_x C_y + A_y B_y C_y + A_z B_z C_y \\
    A_x B_x C_z + A_y B_y C_z + A_z B_z C_z
  \end{bmatrix} \\

  &= \boxed{
    \begin{bmatrix}
      A_y B_x C_y - A_y B_y C_x - A_z B_z C_x + A_z B_x C_z \\
      A_z B_y C_z - A_z B_z C_y - A_x B_x C_y + A_x B_y C_x \\
      A_x B_z C_x - A_x B_x C_z - A_y B_y C_z + A_y B_z C_y
    \end{bmatrix}
  }
\end{align*}
$$

## Problem 1.2

Given:

$$
(A \times B) \cdot (C \times D) = \boxed{(A \cdot C) (B \cdot D) - (A \cdot D) (B \cdot C)}
$$

Using identity (b):

$$
(A \times B) \cdot (C \times D) = ((A \times B) \times C ) \cdot D
$$

Flipping order of cross project:

$$
((A \times B) \times C ) \cdot D = -(C \times (A \times B)) \cdot D
$$

Using identity (c):

$$
C \times (A \times B) = A (C \cdot B) - B (C \cdot A)
$$

Plugging it back in:

$$
-(C \times (A \times B)) \cdot D = -(A (C \cdot B) - B (C \cdot A)) \cdot D
$$

Distribute sign:

$$
-(A (C \cdot B) - B (C \cdot A)) \cdot D = (B (C \cdot A) - A (C \cdot B)) \cdot D
$$

Distribute dot product:

$$
(B \cdot D) (C \cdot A) - (A \cdot D) (C \cdot B)
$$

Rearrange:

$$
(B \cdot D) (C \cdot A) - (A \cdot D) (C \cdot B) = \boxed{(A \cdot C) (B \cdot D) - (A \cdot D) (B \cdot C)}
$$
